fm26.v
@@ -1,0 +1,163 @@
+Require Import FORYU.state.
+Require Import FORYU.program.
+Require Import FORYU.semantics.
+Require Import FORYU.liveness.
+Require Import FORYU.liveness_snd.
+Require Import Orders.
+Require Import OrdersEx.
+Require Import MSets.
+Require Import Arith.
+Require Import List.
+Import ListNotations.
+Require Import Coq.Relations.Relation_Operators.
+Require Import stdpp.prelude.
+Require Import stdpp.relations.
+Require Import Coq.Logic.FunctionalExtensionality.
+Require Import Coq.Logic.Classical_Pred_Type.
+Require Import Lia.
+
+
+Module FM26 (D: DIALECT).
+
+  Module Liveness_sndD := Liveness_snd(D).
+
+  Module LivenessD := Liveness_sndD.LivenessD.
+  Module SmallStepD := LivenessD.SmallStepD.
+  Module StateD := SmallStepD.StateD.
+  Module SmartContractD := SmallStepD.SmartContractD.
+  Module FunctionD := SmartContractD.FunctionD.
+  Module BlockD := SmartContractD.BlockD.
+  Module ExitInfoD := BlockD.ExitInfoD.
+  Module InstructionD := BlockD.InstructionD.
+  Module YULVariableMapD := BlockD.PhiInfoD.YULVariableMapD.
+  Module SimpleExprD := BlockD.PhiInfoD.YULVariableMapD.SimpleExprD.
+  Module CallStackD := StateD.CallStackD.
+  Module StackFrameD := CallStackD.StackFrameD.
+  Module VariableAssignmentD := StackFrameD.VariableAssignmentD.
+
+  Import LivenessD.
+  Import Liveness_sndD.
+
+
+  Definition list_sexp_to_varset (l : list SimpleExprD.t) :=
+    (list_to_set (extract_yul_vars l)).
+  
+  Definition same_pp (fname: FunctionName.t) (bid: BlockID.t) (pc: nat) (sf1 sf2: StackFrameD.t) :=
+    sf1.(StackFrameD.function_name) = fname /\ sf2.(StackFrameD.function_name) = fname /\
+      sf1.(StackFrameD.curr_block_id) = bid /\ sf2.(StackFrameD.curr_block_id) = bid /\ sf1.(StackFrameD.pc) = pc /\ sf2.(StackFrameD.pc) = pc.
+
+  Definition equiv_frames_up_to_v (fname: FunctionName.t) (bid: BlockID.t) (pc: nat)
+    (v: YULVariable.t) (sf1 sf2: StackFrameD.t) :=
+    same_pp fname bid pc sf1 sf2 /\
+      forall v', v' <> v -> (* equality is required for variable different from v *)
+                  VariableAssignmentD.get sf1.(StackFrameD.variable_assignments) v' = VariableAssignmentD.get sf2.(StackFrameD.variable_assignments) v'.
+    
+  Definition equiv_states_up_to_v (fname: FunctionName.t) (bid: BlockID.t) (pc: nat) (v: YULVariable.t) (st1 st2: StateD.t) :=
+    Nat.lt 0 (length (StateD.call_stack st1)) /\
+    length (StateD.call_stack st1) = length (StateD.call_stack st2) /\
+      st1.(StateD.status) = st2.(StateD.status) /\ st1.(StateD.dialect_state) = st2.(StateD.dialect_state) /\ 
+      exists sf1 sf2 rsf,
+        st1.(StateD.call_stack) = sf1::rsf /\ st2.(StateD.call_stack) = sf2::rsf /\
+          equiv_frames_up_to_v fname bid pc v sf1 sf2.
+
+  Definition accessed_vars (b: BlockD.t) (pc: nat) (s: VarSet.t) :=
+  ( pc = (length b.(BlockD.instructions)) /\ (* end of block *)
+    match b.(BlockD.exit_info) with
+    | ExitInfoD.ConditionalJump cv _ _ =>
+       VarSet.Equal s (VarSet.add cv VarSet.empty) (* cv is accessed *)
+    | ExitInfoD.ReturnBlock rvs =>
+       VarSet.Equal s (list_sexp_to_varset rvs) (* rs are accessed *)
+    | _ => VarSet.Equal s VarSet.empty (* nothing is accessed *)
+    end )
+  \/
+  ( pc < (length b.(BlockD.instructions)) /\  (* within the block *)
+    exists instr,                  (* instr.input are accessed *)
+      nth_error b.(BlockD.instructions) pc = Some instr /\
+      (VarSet.Equal s (list_sexp_to_varset instr.(InstructionD.input)) )).
+
+  Definition equiv_top_frame (p: SmartContractD.t) (st1 st2: StateD.t) :=
+  match st1.(StateD.call_stack), st2.(StateD.call_stack) with
+  | nil,nil => True (* both call stacks are empty *)
+  | sf1::_,sf2::_ => (* top frames agree on values of accessed variables *)
+      let fname := sf1.(StackFrameD.function_name) in
+      let bid := sf1.(StackFrameD.curr_block_id) in
+      let pc := sf1.(StackFrameD.pc) in
+        same_pp fname bid pc sf1 sf2 /\
+        forall v s b,
+           SmartContractD.get_block p fname bid = Some b ->
+           Liveness_sndD.accessed_vars b pc s ->
+           VarSet.In v s ->
+           VariableAssignmentD.get sf1.(StackFrameD.variable_assignments) v = VariableAssignmentD.get sf2.(StackFrameD.variable_assignments) v
+  | _,_ => False (* one of the call stacks is empty *)
+ end.
+
+  Definition dead_variable (p: SmartContractD.t) (fname: FunctionName.t) (bid: BlockID.t) (pc: nat) (v: YULVariable.t) :=
+    forall (st1 st2 st1': StateD.t) (n: nat),
+      equiv_states_up_to_v fname bid pc v st1 st2 ->
+      SmallStepD.eval n st1 p = st1' ->
+      exists st2',
+        SmallStepD.eval n st2 p = st2' /\ equiv_top_frame p st1' st2'.
+
+  Lemma equiv_state_rel:
+    forall p fname bid pc v st1 st2,
+      equiv_states_up_to_v fname bid pc v st1 st2 ->
+      equiv_states_up_to_i_v p (length st1.(StateD.call_stack) -1) fname bid pc v st1 st2.
+  Proof.
+    intros p fname bid pc v st1 st2 H_equiv_st1_st2.
+    unfold equiv_states_up_to_i_v.
+    unfold equiv_states_up_to_v in H_equiv_st1_st2.
+    destruct H_equiv_st1_st2 as [H_not_empty [H_len_call_stack [H_status [H_dialect [sf1 [sf2 [rsf [H_call_stack_st1 [H_call_stack_st2 H_equiv_frames]]]]]]]]].
+
+    unfold equiv_frames_up_to_v in H_equiv_frames.
+    unfold same_pp in H_equiv_frames.
+    destruct H_equiv_frames as [ [H_fname_sf1 [H_fname_sf2 [H_bid_sf1 [H_bid_sf2 [H_pc_sf1 H_pc_sf2 ]]]]] H_equiv_varmap].
+     
+    repeat split.
+    - lia.
+    - apply H_len_call_stack.
+    - apply H_status.
+    - apply H_dialect.
+    -  exists [].
+      exists rsf.
+      exists sf1.
+      exists sf2.
+       
+      repeat split; try (assumption || lia).       
+      + rewrite H_call_stack_st1. simpl. lia.
+      + rewrite H_call_stack_st1. simpl. lia.
+  Qed.
+  
+  (*
+     This is an instance of the main lemma live_at_snd in liveness_snd.v.
+  *)
+  Lemma live_in_out_snd:  
+  forall p fname bid b s,
+    SmartContractD.get_block p fname bid = Some b ->
+     live_in p fname bid s ->
+     forall v, ~ VarSet.In v s -> dead_variable p fname bid 0 v.
+  Proof.
+    unfold dead_variable.
+    intros p fname bid b s H_b_exists H_live_in v H_not_In_v_s st1 st2 st1' n H_st1_equiv_st2 H_eval.
+
+    rewrite <- live_at_pc_zero_eq_live_in in H_live_in.
+    apply (live_at_pc'_0_equiv_live_at_pc_0 p fname bid b s H_b_exists) in H_live_in.
+
+    pose proof (equiv_state_rel p fname bid 0%nat v st1 st2 H_st1_equiv_st2) as H_st1_equiv_st2_gen.
+    
+    remember (length st1.(StateD.call_stack)) as i eqn:E_i. 
+    
+    
+    pose proof (live_at_snd p n fname bid b 0%nat s H_b_exists H_live_in st1 st2 st1' v (i-1) H_st1_equiv_st2_gen H_eval H_not_In_v_s) as [st2' [pc' [b' [bid' [H_eval_st2 [H_b'_exists [H_equiv_st1'_st2'_gen H_equiv_top_frame_gen]]]]]]].
+
+    exists st2'.
+    split.
+    - apply H_eval_st2.
+    - unfold equiv_vars_in_top_frame in H_equiv_top_frame_gen.
+      unfold equiv_top_frame. 
+      destruct (StateD.call_stack st1') as [|sf1' rs1']; try assumption.
+      destruct (StateD.call_stack st2') as [|sf2' rs2']; try assumption.
+      destruct H_equiv_top_frame_gen as [H_fname_sf1'_sf2' [H_bid_sf1'_sf2' [H_pc_sf1'_sf2' H_equiv_varmap]]].
+      unfold same_pp.       
+      repeat split; try (assumption || intuition).
+  Qed.
+End FM26.
